clight/interpreter.v
@@ -2395,7 +2395,7 @@ Definition f_step_opcode_mem_st_imm := {|
   fn_return := tvoid;
   fn_callconv := cc_default;
   fn_params := ((_st, (tptr (Tstruct _bpf_state noattr))) :: (_imm, tint) ::
-                (_addr, tuint) :: (_dst, tuint) :: (_op, tuchar) :: nil);
+                (_addr, tuint) :: (_op, tuchar) :: nil);
   fn_vars := nil;
   fn_temps := ((_opcode_st, tuchar) :: (_addr_ptr, (tptr tuchar)) ::
                (_is_null, tbool) :: (_t'9, tbool) :: (_t'8, (tptr tuchar)) ::
@@ -2608,8 +2608,7 @@ Definition f_step_opcode_mem_st_reg := {|
   fn_return := tvoid;
   fn_callconv := cc_default;
   fn_params := ((_st, (tptr (Tstruct _bpf_state noattr))) ::
-                (_src64, tulong) :: (_addr, tuint) :: (_dst, tuint) ::
-                (_op, tuchar) :: nil);
+                (_src64, tulong) :: (_addr, tuint) :: (_op, tuchar) :: nil);
   fn_vars := nil;
   fn_temps := ((_opcode_st, tuchar) :: (_addr_ptr, (tptr tuchar)) ::
                (_is_null, tbool) :: (_t'9, tbool) :: (_t'8, (tptr tuchar)) ::
@@ -3159,16 +3158,13 @@ Definition f_step := {|
                                                                     (Tcons
                                                                     tuint
                                                                     (Tcons
-                                                                    tuint
-                                                                    (Tcons
                                                                     tuchar
-                                                                    Tnil)))))
+                                                                    Tnil))))
                                                                     tvoid
                                                                     cc_default))
                                     ((Etempvar _st (tptr (Tstruct _bpf_state noattr))) ::
                                      (Etempvar _imm tint) ::
                                      (Etempvar _addr tuint) ::
-                                     (Etempvar _dst tuint) ::
                                      (Etempvar _op tuchar) :: nil))
                                   (Sreturn None))))))
                         (LScons (Some 3)
@@ -3230,13 +3226,11 @@ Definition f_step := {|
                                             (tptr (Tstruct _bpf_state noattr))
                                             (Tcons tulong
                                               (Tcons tuint
-                                                (Tcons tuint
-                                                  (Tcons tuchar Tnil)))))
-                                          tvoid cc_default))
+                                                (Tcons tuchar Tnil)))) tvoid
+                                          cc_default))
                                         ((Etempvar _st (tptr (Tstruct _bpf_state noattr))) ::
                                          (Etempvar _src64 tulong) ::
                                          (Etempvar _addr tuint) ::
-                                         (Etempvar _dst tuint) ::
                                          (Etempvar _op tuchar) :: nil))
                                       (Sreturn None)))))))
                           (LScons None
