monadicmodel/rBPFInterpreter.v
@@ -398,7 +398,7 @@ Definition step_opcode_mem_ld_reg (addr: val) (dst: reg) (op: nat): M state unit
   | op_BPF_LDX_REG_ILLEGAL_INS => upd_flag BPF_ILLEGAL_INSTRUCTION
   end.
 
-Definition step_opcode_mem_st_imm (imm: val) (addr: val) (dst: reg) (op: nat): M state unit :=
+Definition step_opcode_mem_st_imm (imm: val) (addr: val) (op: nat): M state unit :=
   do opcode_st <- get_opcode_mem_st_imm op;
   match opcode_st with
   | op_BPF_STW       =>
@@ -432,7 +432,7 @@ Definition step_opcode_mem_st_imm (imm: val) (addr: val) (dst: reg) (op: nat): M
   | op_BPF_ST_IMM_ILLEGAL_INS => upd_flag BPF_ILLEGAL_INSTRUCTION
   end.
 
-Definition step_opcode_mem_st_reg (src64: val) (addr: val) (dst: reg) (op: nat): M state unit :=
+Definition step_opcode_mem_st_reg (src64: val) (addr: val) (op: nat): M state unit :=
   do opcode_st <- get_opcode_mem_st_reg op;
   match opcode_st with
   | op_BPF_STXW      =>
@@ -505,14 +505,14 @@ Definition step: M state unit :=
     do ofs    <- get_offset ins;
     do imm    <- get_immediate ins;
     do addr   <- get_addr_ofs dst64 ofs;
-    step_opcode_mem_st_imm (sint32_to_vint imm) addr dst op       (**r 0xX2/0xXa *)
+    step_opcode_mem_st_imm (sint32_to_vint imm) addr op       (**r 0xX2/0xXa *)
   | op_BPF_Mem_st_reg  =>
     do dst64  <- eval_reg dst;
     do src    <- get_src ins;
     do src64  <- eval_reg src;
     do ofs    <- get_offset ins;
     do addr <- get_addr_ofs dst64 ofs;
-    step_opcode_mem_st_reg src64 addr dst op       (**r 0xX3/0xXb *)
+    step_opcode_mem_st_reg src64 addr op       (**r 0xX3/0xXb *)
   | op_BPF_ILLEGAL_INS => upd_flag BPF_ILLEGAL_INSTRUCTION
   end.
 
