simulation/correct_step_opcode_branch.v
@@ -16,7 +16,7 @@
 (*                                                                        *)
 (**************************************************************************)
 
-From bpf.comm Require Import Regs State Monad rBPFMonadOp.
+From bpf.comm Require Import Flag Regs State Monad rBPFMonadOp.
 From bpf.monadicmodel Require Import rBPFInterpreter.
 From bpf.monadicmodel Require Import Opcode.
 From Coq Require Import List Lia ZArith.
